Context.stlc_subst_ctx

LogicalRefinement/Stlc/Interp.lean
@@ -67,6 +67,22 @@ def Context.stlc: Context -> Stlc.Context
 | [] => []
 | H::Hs => H.stlc::(stlc Hs)
 
+def Context.stlc_strict: Context -> Stlc.Context
+| [] => []
+| (Hyp.mk A (HypKind.val type))::Hs => A.stlc_ty::(stlc Hs)
+| H::Hs => stlc Hs
+
+def Context.stlc_subst: (Γ: Context) -> Stlc.Subst
+| [] => (λn => Stlc.var n)
+| (Hyp.mk A (HypKind.val type))::Hs => (stlc_subst Hs).lift
+| H::Hs => (λn => match n with
+                  | 0 => Stlc.abort
+                  | Nat.succ n => stlc_subst Hs n)
+
+theorem Context.stlc_subst_ctx {Γ: Context}
+  : Stlc.SubstCtx Γ.stlc_subst Γ.stlc_strict Γ.stlc
+  := by sorry
+
 theorem HasType.stlc_ty_subst {Γ A σ s} (H: Γ ⊢ A: sort s):
   (A.subst σ).stlc_ty = A.stlc_ty := by {
   revert H s σ Γ;
